define model

model.v
@@ -3,23 +3,64 @@ Require Import Program.
 Require Import category.
 Require Import stlc.
 
-Fixpoint ty_denot {C} `{CartesianClosed C} (t : type) : C :=
+Fixpoint ty_denot {C : Type} `{CartesianClosed C} (t : type) : C :=
   match t with
   | unit_type => terminal_obj
   | prod_type t1 t2 => product (ty_denot t1) (ty_denot t2)
   | arrow_type t1 t2 => exponential (ty_denot t1) (ty_denot t2)
   end.
 
-Fixpoint ctx_denot {C} `{CartesianClosed C} (Γ : context) : C :=
+Fixpoint ctx_denot {C : Type} `{CartesianClosed C} (Γ : context) : C :=
   match Γ with
   | empty_context => terminal_obj
-  | context_cons t Γ => product (ty_denot t) (ctx_denot Γ) 
+  | context_cons t Γ => product (ctx_denot Γ) (ty_denot t)
   end.
+
+Fixpoint var_denot {C: Type} `{CartesianClosed C} {Γ t} (x : contains Γ t) : Hom (ctx_denot Γ) (ty_denot t).
+Proof.
+  destruct x eqn:Hx.
+  + refine snd.
+  + eapply compose.
+    - apply var_denot.
+      refine c.
+    - refine fst.
+Defined.
 
 Fixpoint tm_denot {C} `{CartesianClosed C} {Γ t} (e : term Γ t)
 : Hom (ctx_denot Γ) (ty_denot t).
 Proof.
-  destruct e.
+  destruct e eqn:He.
+  + refine terminal_map.
+  + simpl ty_denot.
+    apply f_prod.
+    - apply tm_denot.
+      assumption.
+    - apply tm_denot.
+      assumption.
+  + eapply compose.
+    2:{
+      refine (tm_denot _ _ _ _ _ _ _ _ t0).
+    }
+    - refine fst.
+  + eapply compose.
+    2:{
+      refine (tm_denot _ _ _ _ _ _ _ _ t0).
+    }
+    - refine snd.
+  + apply var_denot.
+    refine c.
   + simpl.
-
-Admitted.
+    apply curry.
+    replace (product (ctx_denot Γ) (ty_denot t1)) with (ctx_denot (context_cons t1 Γ)) by reflexivity.
+    apply tm_denot.
+    refine t0.
+  + eapply compose.
+    2:{
+      eapply f_prod.
+      + apply tm_denot.
+        refine t0_1.
+      + apply tm_denot.
+        refine t0_2.
+    }
+    apply eval.
+Defined.
